Fix after relaxed Add/SubOverflow conditions

compiler/backend/semantics/wordPropsScript.sml
@@ -2241,9 +2241,9 @@ val inst_ok_less_def = Define`
   (inst_ok_less c (Arith (AddCarry r1 r2 r3 r4)) =
      (((c.ISA = MIPS) \/ (c.ISA = RISC_V)) ==> r1 ≠ r3 /\ r1 ≠ r4)) ∧
   (inst_ok_less c (Arith (AddOverflow r1 r2 r3 r4)) =
-     (((c.ISA = MIPS) \/ (c.ISA = RISC_V)) ==> r1 ≠ r2 /\ r1 ≠ r3)) ∧
+     (((c.ISA = MIPS) \/ (c.ISA = RISC_V)) ==> r1 ≠ r3)) ∧
   (inst_ok_less c (Arith (SubOverflow r1 r2 r3 r4)) =
-     (((c.ISA = MIPS) \/ (c.ISA = RISC_V)) ==> r1 ≠ r2 /\ r1 ≠ r3)) ∧
+     (((c.ISA = MIPS) \/ (c.ISA = RISC_V)) ==> r1 ≠ r3)) ∧
   (inst_ok_less c (Mem m r (Addr r' w)) =
     addr_offset_ok w c) ∧
   (inst_ok_less _ _ = T)`
@@ -2336,8 +2336,8 @@ val wf_cutsets_def = Define`
 val inst_arg_convention_def = Define`
   (inst_arg_convention (Arith (AddCarry r1 r2 r3 r4)) ⇔ r4 = 0) ∧
   (* Note: these are not necessary *)
-  (inst_arg_convention (Arith (AddOverflow r1 r2 r3 r4)) ⇔ r2 = 2 ∧ r4 = 0) ∧
-  (inst_arg_convention (Arith (SubOverflow r1 r2 r3 r4)) ⇔ r2 = 2 ∧ r4 = 0) ∧
+  (inst_arg_convention (Arith (AddOverflow r1 r2 r3 r4)) ⇔ r4 = 0) ∧
+  (inst_arg_convention (Arith (SubOverflow r1 r2 r3 r4)) ⇔ r4 = 0) ∧
   (* Follows conventions for x86 *)
   (inst_arg_convention (Arith (LongMul r1 r2 r3 r4)) ⇔ r1 = 8 ∧ r2 = 0 ∧ r3 = 0 ∧ r4 = 4) ∧
   (inst_arg_convention (Arith (LongDiv r1 r2 r3 r4 r5)) ⇔ r1 = 0 ∧ r2 = 8 ∧ r3 = 0 ∧ r4 = 8) ∧
