compiler/backend/word_allocScript.sml
@@ -132,19 +132,17 @@ val ssa_cc_trans_inst_def = Define`
     let r2' = option_lookup ssa r2 in
     let r3' = option_lookup ssa r3 in
     (* TODO: This might need to be made a strong preference *)
-    let mov_in = Move 0 [(2,r2')] in
     let (r1',ssa',na') = next_var_rename r1 ssa na in
     let (r4'',ssa'',na'') = next_var_rename r4 ssa' na' in
     let mov_out = Move 0 [(r4'',0)] in
-      (Seq mov_in (Seq (Inst (Arith (AddOverflow r1' 2 r3' 0))) mov_out), ssa'',na'')) ∧
+      (Seq (Inst (Arith (AddOverflow r1' r2' r3' 0))) mov_out, ssa'',na'')) ∧
   (ssa_cc_trans_inst (Arith (SubOverflow r1 r2 r3 r4)) ssa na =
     let r2' = option_lookup ssa r2 in
     let r3' = option_lookup ssa r3 in
-    let mov_in = Move 0 [(2,r2')] in
     let (r1',ssa',na') = next_var_rename r1 ssa na in
     let (r4'',ssa'',na'') = next_var_rename r4 ssa' na' in
     let mov_out = Move 0 [(r4'',0)] in
-      (Seq mov_in (Seq (Inst (Arith (SubOverflow r1' 2 r3' 0))) mov_out), ssa'',na'')) ∧
+      (Seq (Inst (Arith (SubOverflow r1' r2' r3' 0))) mov_out, ssa'',na'')) ∧
   (ssa_cc_trans_inst (Arith (LongMul r1 r2 r3 r4)) ssa na =
     let r3' = option_lookup ssa r3 in
     let r4' = option_lookup ssa r4 in
@@ -781,13 +779,11 @@ val get_forced_def = Define`
        else acc
     | Arith (AddOverflow r1 r2 r3 r4) =>
        if (c.ISA = MIPS ∨ c.ISA = RISC_V) then
-          (if r1=r2 then [] else [(r1,r2)]) ++
           (if r1=r3 then [] else [(r1,r3)]) ++
           acc
        else acc
     | Arith (SubOverflow r1 r2 r3 r4) =>
        if (c.ISA = MIPS ∨ c.ISA = RISC_V) then
-          (if r1=r2 then [] else [(r1,r2)]) ++
           (if r1=r3 then [] else [(r1,r3)]) ++
           acc
        else acc
